Checkpoint tutorial proof progress

src/program_proof/tutorial/objectstore/proof.v
@@ -1,4 +1,6 @@
 From Perennial.program_proof Require Import grove_prelude.
+From Goose.github_com.mit_pdos.gokv.tutorial.objectstore Require Export chunk dir client.
+From Perennial.base_logic.lib Require Import ghost_map.
 
 (*
   map keyname → chunkhandle
@@ -42,3 +44,139 @@ From Perennial.program_proof Require Import grove_prelude.
        Hash(content)
       { content_hash:string, RET #content_hash; content_hash ↦[γhash]□ content }
 *)
+
+Module PreparedWrite.
+Record t := mk
+  {
+    Id: u64;
+    ChunkAddrs: list chan;
+  }.
+
+End PreparedWrite.
+
+Module RecordChunkArgs.
+  Record t := mk
+    {
+      WriteId: u64;
+      Index: u64;
+      Server: chan;
+      ContentHash: string;
+    }.
+End RecordChunkArgs.
+
+Module FinishWriteArgs.
+  Record t := mk
+    {
+      WriteId: u64;
+      Keyname: string;
+    }.
+End FinishWriteArgs.
+
+Section proof.
+
+Context `{!heapGS Σ}.
+Context `{ghost_mapG Σ nat (chan * list u8)}.
+Context `{ghost_mapG Σ (u64 * nat) unit}.
+
+Record dir_names :=
+  {
+    writeId_gn:gname; (* ghost_map writeId → gname *)
+    recorded_gn:gname; (* ghost_map (writeId:u64, index:nat) → unit *)
+  }
+.
+
+Definition own_PreparedWrite (v:val) (x:PreparedWrite.t) : iProp Σ :=
+  ∃ (addrs_sl:Slice.t),
+  ⌜v = (#x.(PreparedWrite.Id), (slice_val addrs_sl, #() ))%V⌝ ∗
+  readonly (is_slice_small addrs_sl uint64T 1%Qp x.(PreparedWrite.ChunkAddrs))
+  (* [∗ list] index ↦ '(addr, _) ∈ chunkhandles, is_chunk_host γchunk? addr *)
+.
+
+Implicit Type γd : dir_names.
+
+(* This owned by the client, and is used to decide what the data for this WriteID will be *)
+Definition own_WriteId γd (id:u64) (chunkhandles:list (chan * (list u8) )) : iProp Σ :=
+  (* id + γ should determine the γid *)
+  ∃ γid, ghost_map_auth γid 1 (map_seq 0 chunkhandles)
+  (* [∗ list] index ↦ v ∈ chunkhandles, index ↪[γ] v *)
+  (* [∗ list] index ↦ '(addr, _) ∈ chunkhandles, is_chunk_host γchunk? addr *)
+.
+
+Definition is_Clerk (ck:loc) γd : iProp Σ := True.
+
+Lemma wp_Clerk__PrepareWrite (ck:loc) γd :
+  {{{
+        is_Clerk ck γd
+  }}}
+    Clerk__PrepareWrite #ck
+  {{{
+        v x, RET v; own_PreparedWrite v x ∗
+                     own_WriteId γd x.(PreparedWrite.Id) []
+  }}}
+.
+Proof.
+Admitted.
+
+(* This is a witness that the client has decided on the data/server at an index for a writeId *)
+Definition is_client_writeId_index γd (id:u64) (index:nat) (chunkhandle:chan * list u8) : iProp Σ :=
+  ∃ γid, (* id + γ should determine the γid *)
+  index ↪[γid]□ chunkhandle
+.
+
+Lemma decide_writeId_index γd (id:u64) chunkhandles newchunkhandle :
+  own_WriteId γd id chunkhandles ==∗
+  own_WriteId γd id (chunkhandles ++ [newchunkhandle]) ∗
+  is_client_writeId_index γd id (length chunkhandles) newchunkhandle.
+Proof.
+Admitted.
+
+Definition is_dir_writeId_index_recorded γd (id:u64) (index:nat) : iProp Σ :=
+  (id, index) ↪[γd.(recorded_gn)]□ ()
+.
+
+Lemma wp_Clerk__RecordChunk γd (ck:loc) args data :
+  {{{
+        is_Clerk ck γd ∗
+        is_client_writeId_index γd args.(RecordChunkArgs.WriteId) (int.nat args.(RecordChunkArgs.Index))
+                           (args.(RecordChunkArgs.Server), data)
+        (* own args *)
+        (* witness that args.(RecordChunkArgs.Server) stores data with args.(RecordChunkArgs.ContentHash) *)
+  }}}
+    Clerk__RecordChunk #ck (* #args *)
+  {{{
+        RET #(); is_dir_writeId_index_recorded γd args.(RecordChunkArgs.WriteId)
+                                                         (int.nat args.(RecordChunkArgs.Index))
+  }}}
+.
+Proof.
+Admitted.
+
+Definition is_finished_writeId γd (id:u64) chunkhandles : iProp Σ :=
+  (* XXX: should be able to to have DfracDiscarded in place of (1:Qp) *)
+  ∃ γid, readonly (ghost_map_auth γid 1 (map_seq 0 chunkhandles))
+.
+
+Definition object_ptsto γd (key:string) (data:list (list u8)) : iProp Σ :=
+ True
+.
+
+(* The code is not exactly-once because FinishWrite might run many times. The
+   spec cannot take and return ownership of the object_ptsto. *)
+Lemma wp_Clerk__FinishWrite γd (ck:loc) args chunkhandles (data newdata : list (list u8)) :
+  {{{
+        is_Clerk ck γd ∗
+        is_finished_writeId γd args.(FinishWriteArgs.WriteId) chunkhandles ∗
+        ([∗ list] index ↦ _ ∈ chunkhandles,
+          is_dir_writeId_index_recorded γd args.(FinishWriteArgs.WriteId) index) ∗
+        ⌜chunkhandles.*2 = newdata⌝ ∗
+        object_ptsto γd args.(FinishWriteArgs.Keyname) data
+  }}}
+    Clerk__FinishWrite #ck (* #args *)
+  {{{
+        RET #(); object_ptsto γd args.(FinishWriteArgs.Keyname) newdata
+  }}}
+.
+Proof.
+Admitted.
+
+End proof.
